replaced CM2 by MM2 in reversible halting, uniform boundedness, and uniform mortality added MM2_dec

theories/MinskyMachines/MM2.v
@@ -1,95 +1,169 @@
-(**************************************************************)
-(*   Copyright Dominique Larchey-Wendling [*]                 *)
-(*                                                            *)
-(*                             [*] Affiliation LORIA -- CNRS  *)
-(**************************************************************)
-(*      This file is distributed under the terms of the       *)
-(*         CeCILL v2 FREE SOFTWARE LICENSE AGREEMENT          *)
-(**************************************************************)
+(* 
+  Author(s):
+    Dominique Larchey-Wendling (1)
+    Andrej Dudenhefner (2)
+  Affiliation(s):
+    (1) LORIA -- CNRS
+    (2) TU Dortmund University, Dortmund, Germany
+*)
 
-(* Certified Undecidability of Intuitionistic Linear Logic via Binary Stack Machines and Minsky Machines. Yannick Forster and Dominique Larchey-Wendling. CPP '19. http://uds-psl.github.io/ill-undecidability/ *)
+(* 
+  Problem(s):
+    Two-counter Machine Halting (MM2_HALTING)
+    Two-counter Machine Halting starting from (0, 0) (MM2_ZERO_HALTING)
+    Two-counter Machine Halting ending in (0, 0) (MM2_HALTS_ON_ZERO)
+    Two-counter Machine Reversibility (MM2_REV)
+    Reversible Two-counter Machine Halting (MM2_REV_HALT)
+    Two-counter Machine Uniform Boundedness (MM2_UBOUNDED)
+    Two-counter Machine Uniform Mortality (MM2_UMORTAL)
+*)
 
-(** * Halting problem for two counter Minsky machines MM2_HALTING  *)
+(* 
+  Literature:
+  [1] Certified Undecidability of Intuitionistic Linear Logic via Binary Stack Machines and Minsky Machines.
+      Yannick Forster and Dominique Larchey-Wendling. CPP '19. http://uds-psl.github.io/ill-undecidability/ 
+*)
 
-Require Import Relations.Relation_Operators.
-#[local] Open Scope list_scope.
+Require Import List Relations.Relation_Operators.
 
-Set Implicit Arguments.
+#[local] Set Implicit Arguments.
 
-Section self_contained_mm2.
+(* Two counters Minsky machines. Counters are named A and B
 
-  (* Two counters Minsky machines. Counters are named A and B
+    For instructions: INC{A,B} | DEC{A,B} j 
 
-      For instructions: INC{A,B} | DEC{A,B} j 
+    j is a conditional jump PC index which occurs
+    when the counter has non-zero value 
+*)
 
-      j is a conditional jump PC index which occurs
-      when the counter has non-zero value 
+Inductive mm2_instr : Set :=
+  | mm2_inc_a : mm2_instr
+  | mm2_inc_b : mm2_instr
+  | mm2_dec_a : nat -> mm2_instr
+  | mm2_dec_b : nat -> mm2_instr.
+
+Reserved Notation "i '//' r '⇢' s" (at level 70, no associativity).
+Reserved Notation "P '//' r '→' s" (at level 70, no associativity).
+Reserved Notation "P '//' r '↠' s" (at level 70, no associativity).
+Reserved Notation "P '//' r ↓" (at level 70, no associativity).
+
+#[local] Notation mm2_state := (nat*(nat*nat))%type.
+
+(* Instruction step semantics:
+
+    ρ // x ⇢ y : instruction ρ transforms state x into state y 
+
+    Notice that the jump occurs on the non-zero case when DEC
+
   *)
 
-  Inductive mm2_instr : Set :=
-    | mm2_inc_a : mm2_instr
-    | mm2_inc_b : mm2_instr
-    | mm2_dec_a : nat -> mm2_instr
-    | mm2_dec_b : nat -> mm2_instr.
+Inductive mm2_atom : mm2_instr -> mm2_state -> mm2_state -> Prop :=
+  | in_mm2s_inc_a  : forall i   a b, mm2_inc_a   // (i,(  a,  b)) ⇢ (1+i,(S a,  b))
+  | in_mm2s_inc_b  : forall i   a b, mm2_inc_b   // (i,(  a,  b)) ⇢ (1+i,(  a,S b))
+  | in_mm2s_dec_aS : forall i j a b, mm2_dec_a j // (i,(S a,  b)) ⇢ (  j,(  a,  b))
+  | in_mm2s_dec_bS : forall i j a b, mm2_dec_b j // (i,(  a,S b)) ⇢ (  j,(  a,  b))
+  | in_mm2s_dec_a0 : forall i j   b, mm2_dec_a j // (i,(  0,  b)) ⇢ (1+i,(  0,  b))
+  | in_mm2s_dec_b0 : forall i j a,   mm2_dec_b j // (i,(  a,  0)) ⇢ (1+i,(  a,  0))
+where "ρ // x ⇢ y" := (mm2_atom ρ x y).
 
-  Reserved Notation "i '//' r '⇢' s" (at level 70, no associativity).
-  Reserved Notation "P '//' r '→' s" (at level 70, no associativity).
-  Reserved Notation "P '//' r '↠' s" (at level 70, no associativity).
-  Reserved Notation "P '//' r ↓" (at level 70, no associativity).
+(* instruction ρ occurs at PC index i in the program (1,P) *)
 
+Definition mm2_instr_at (ρ : mm2_instr) i P := exists l r, P = l++ρ::r /\ 1+length l = i.
+
+(* Program step semantics:
+
+    program P with first instruction at PC index 1 transforms 
+    state x into state y in one step, using instruction a PC index (fst x) *)
+
+Definition mm2_step P x y := exists ρ, mm2_instr_at ρ (fst x) P /\ ρ // x ⇢ y.
+#[local] Notation "P // x → y" := (mm2_step P x y).
+
+(* Halting condition: program P cannot progress from s *)
+Definition mm2_stop P s := forall s', not (P // s → s').
+
+(* reflexive and transitive closure of program step semantics *)
+#[local] Notation "P // x ↠ y" := (clos_refl_trans _ (mm2_step P) x y).
+
+Definition mm2_terminates P s := exists s', P // s ↠ s' /\ mm2_stop P s'.
+#[local] Notation "P // s ↓" := (mm2_terminates P s).
+
+Definition MM2_PROBLEM := (list mm2_instr * nat * nat)%type.
+
+(* Two-counter Machine Halting *)
+Definition MM2_HALTING (P : MM2_PROBLEM) := 
+  match P with (P,a,b) => P // (1,(a,b)) ↓ end.
+
+(* Two-counter Machine Halting starting from (0, 0) *)
+Definition MM2_ZERO_HALTING : list mm2_instr -> Prop := 
+  fun P => P // (1,(0,0)) ↓.
+
+(* Two-counter Machine Halting ending in (0, 0) *)
+Definition MM2_HALTS_ON_ZERO (P : MM2_PROBLEM) := 
+  match P with (P,a,b) => P // (1,(a,b)) ↠ (0,(0,0)) end.
+
+(* injectivity of the step relation *)
+Definition mm2_reversible (P : list mm2_instr) : Prop := 
+  forall x y z, mm2_step P x z -> mm2_step P y z -> x = y.
+
+(* k bounds the number of reachable configurations from x *)
+Definition mm2_bounded (P : list mm2_instr) (k: nat) (x: mm2_state) : Prop := 
+  exists (L: list mm2_state), (length L <= k) /\
+    (forall (y: mm2_state), P // x ↠ y -> In y L).
+
+(* uniform bound for number of reachable configurations *)
+Definition mm2_uniformly_bounded (P : list mm2_instr) : Prop :=
+  exists k, forall x, mm2_bounded P k x.
+
+(* configuration trace P // x → x1 → x2 → ... → xn *)
+Fixpoint mm2_trace (P : list mm2_instr) (x : mm2_state) (xs : list mm2_state) : Prop :=
+  match xs with
+  | nil => True
+  | y::ys => P // x → y /\ mm2_trace P y ys
+  end.
+
+(* k bounds the number of steps in any run from x *)
+Definition mm2_mortal (P : list mm2_instr) (k: nat) (x: mm2_state) : Prop :=
+  forall (L: list mm2_state), mm2_trace P x L -> length L <= k.
+
+(* uniform bound for number of steps until termination *)
+Definition mm2_uniformly_mortal (P : list mm2_instr) : Prop :=
+  exists k, forall x, mm2_mortal P k x.
+
+(* Two-counter Machine Reversibility:
+   Given a two-counter machine P,
+   is the step function of P injective? *)
+Definition MM2_REV : list mm2_instr -> Prop :=
+  fun P => mm2_reversible P.
+
+(* Reversible Two-counter Machine Halting:
+   Given a reversible two-counter machine P and a configucation x,
+   does a run in M starting from x eventually halt? *)
+Definition MM2_REV_HALT : { P: list mm2_instr | mm2_reversible P } * mm2_state -> Prop :=
+  fun '((exist _ P _), x) => P // x ↓.
+
+(* Two-counter Machine Uniform Boundedness:
+   Given a two-counter machine P,
+   is there a uniform bound n,
+   such that for any configuration x,
+   the number of reacheable configurations from x in P is bounded by n? *)
+Definition MM2_UBOUNDED : list mm2_instr -> Prop :=
+  fun P => mm2_uniformly_bounded P.
+
+(* Two-counter Machine Uniform Mortality:
+   Given a two-counter machine P,
+   is there a uniform bound n,
+   such that for any configuration x,
+   a run in P starting from x halts after at most n steps? *)
+Definition MM2_UMORTAL : list mm2_instr -> Prop :=
+  fun P => mm2_uniformly_mortal P.
+
+Module MM2Notations.
   Notation mm2_state := (nat*(nat*nat))%type.
-
-  (* Instruction step semantics:
-
-      ρ // x ⇢ y : instruction ρ transforms state x into state y 
-
-      Notice that the jump occurs on the non-zero case when DEC
-
-   *)
-
-  Inductive mm2_atom : mm2_instr -> mm2_state -> mm2_state -> Prop :=
-    | in_mm2s_inc_a  : forall i   a b, mm2_inc_a   // (i,(  a,  b)) ⇢ (1+i,(S a,  b))
-    | in_mm2s_inc_b  : forall i   a b, mm2_inc_b   // (i,(  a,  b)) ⇢ (1+i,(  a,S b))
-    | in_mm2s_dec_aS : forall i j a b, mm2_dec_a j // (i,(S a,  b)) ⇢ (  j,(  a,  b))
-    | in_mm2s_dec_bS : forall i j a b, mm2_dec_b j // (i,(  a,S b)) ⇢ (  j,(  a,  b))
-    | in_mm2s_dec_a0 : forall i j   b, mm2_dec_a j // (i,(  0,  b)) ⇢ (1+i,(  0,  b))
-    | in_mm2s_dec_b0 : forall i j a,   mm2_dec_b j // (i,(  a,  0)) ⇢ (1+i,(  a,  0))
-  where "ρ // x ⇢ y" := (mm2_atom ρ x y).
-
-  (* instruction ρ occurs at PC index i in the program (1,P) *)
-
-  Definition mm2_instr_at (ρ : mm2_instr) i P := exists l r, P = l++ρ::r /\ 1+length l = i.
-
-  (* Program step semantics:
-
-      program P with first instruction at PC index 1 transforms 
-      state x into state y in one step, using instruction a PC index (fst x) *)
-
-  Definition mm2_step P x y := exists ρ, mm2_instr_at ρ (fst x) P /\ ρ // x ⇢ y.
-
+  Notation index x := (@fst nat (nat*nat) x).
+  Notation value1 x := (fst (@snd nat (nat*nat) x)).
+  Notation value2 x := (snd (@snd nat (nat*nat) x)).
+  Notation "ρ // x ⇢ y" := (mm2_atom ρ x y).
   Notation "P // x → y" := (mm2_step P x y).
- 
-  (* Halting condition: program P cannot progress anymore *)
-
-  Definition mm2_stop P s := forall s', ~ P // s → s'.
-
-  (* reflexive and transitive closure of program step semantics *)
-
   Notation "P // x ↠ y" := (clos_refl_trans _ (mm2_step P) x y).
-
-  Definition mm2_terminates P s := exists s', P // s ↠ s' /\ mm2_stop P s'.
-
   Notation "P // s ↓" := (mm2_terminates P s).
-
-  Definition MM2_PROBLEM := (list mm2_instr * nat * nat)%type.
-
-  Definition MM2_HALTING (P : MM2_PROBLEM) := 
-    match P with (P,a,b) => P // (1,(a,b)) ↓ end.
-
-  Definition MM2_ZERO_HALTING : list mm2_instr -> Prop := 
-    fun P => P // (1,(0,0)) ↓.
-
-  Definition MM2_HALTS_ON_ZERO (P : MM2_PROBLEM) := 
-    match P with (P,a,b) => P // (1,(a,b)) ↠ (0,(0,0)) end.
-
-End self_contained_mm2.
+End MM2Notations.
