theories/MinskyMachines/Deciders/MM2_REV_dec.v
@@ -1,0 +1,169 @@
+(*
+  Author(s):
+    Andrej Dudenhefner (1)
+  Affiliation(s):
+    (1) TU Dortmund University, Dortmund, Germany
+*)
+
+(*
+  Decision Procedure(s):
+    Two-counter Machine Reversibility (MM2_REV)
+
+  References:
+  [1] Dudenhefner, Andrej. "Certified Decision Procedures for Two-Counter Machines."
+      FSCD 2022. https://drops.dagstuhl.de/opus/volltexte/2022/16297/
+*)
+
+Require Import List ListDec PeanoNat Lia Operators_Properties.
+Import ListNotations.
+Require Import Undecidability.MinskyMachines.MM2.
+Require Import Undecidability.MinskyMachines.Util.MM2_facts.
+Import MM2Notations.
+
+Require Import ssreflect ssrbool ssrfun.
+
+Set Default Goal Selector "!".
+
+(* local facts *)
+Module Facts.
+
+(* transforms a goal (A -> B) -> C into goals A and B -> C *)
+Lemma unnest : forall (A B C : Type), A -> (B -> C) -> (A -> B) -> C.
+Proof. auto. Qed.
+
+End Facts.
+
+Import Facts.
+
+Section Construction.
+Variable M : list mm2_instr.
+
+#[local] Notation step := (mm2_step M).
+#[local] Notation l := (length M).
+
+(* characterize reversibility via a finite number of configurations *)
+Lemma finite_characterization : let t := list_prod (seq 1 l) (list_prod [0;1;2] [0;1;2]) in
+  Forall (fun '(x, y) => forall z, step x z -> step y z -> x = y) (list_prod t t) ->
+  mm2_reversible M.
+Proof.
+  move=> t. pose P := fun '(x, y) => x <> y /\ exists z, step x z /\ step y z.
+  have := Exists_dec P (list_prod t t).
+  apply: unnest.
+  { move=> [x y]. rewrite /P.
+    have [<-|?] := mm2_state_eq_dec x y.
+    { right. tauto. }
+    have [[z1 Hxz1]|Hx] := mm2_sig_step_dec M x.
+    - have [[z2 Hyz2]|Hy] := mm2_sig_step_dec M y.
+      + have [?|?] := mm2_state_eq_dec z2 z1.
+        * left. subst z2. split; [done|]. by exists z1.
+        * right => - [?] [? []].
+          move: Hxz1 => /mm2_step_det /[apply] <-.
+          by move: Hyz2 => /mm2_step_det /[apply].
+      + by right => - [_ [?]] [_ /Hy].
+    - by right => - [_ [?]] [/Hx]. }
+  case.
+  { move=> /Exists_exists [[x y]] [Hxyt] [H1Pxy [z [Hxz Hyz]]].
+    by move=> /Forall_forall /(_ (x, y) Hxyt) /(_ z Hxz Hyz). }
+  move=> /Forall_Exists_neg /Forall_forall HP _.
+  have H''P : forall i j p1 a1 b1 p2 a2 b2 z, mm2_instr_at i p1 M -> mm2_instr_at j p2 M ->
+    0 <= a1 <= 2 /\ 0 <= b1 <= 2 /\ 0 <= a2 <= 2 /\ 0 <= b2 <= 2 -> (p1, (a1, b1)) <> (p2, (a2, b2)) ->
+    mm2_atom i (p1, (a1, b1)) z -> mm2_atom j (p2, (a2, b2)) z -> False.
+  { move=> i j p1 a1 b1 p2 a2 b2 z /[dup] ? /mm2_instr_at_bounds Hi /[dup] ? /mm2_instr_at_bounds Hj *.
+    apply: (HP ((p1, (a1, b1)), (p2, (a2, b2)))).
+    - apply /in_prod; (apply /in_prod; [apply /in_seq|apply /in_prod]).
+      all: move=> /=; lia.
+    - split; [done|].
+      eexists. by split; eexists; split; eassumption. }
+  move=> x y z [i] [Hi Hxz] [j] [Hj].
+  move Ezz': (z) => z' Hyz'.
+  have Hij : fst x = fst y -> i = j.
+  { move=> Hxy. move: Hxy Hi Hj => ->. by apply: mm2_instr_at_unique. }
+  move: (Hi) (Hj) => /H''P /[apply] {}H''P.
+  move: Hxz Hyz' Ezz' Hij Hi Hj H''P.
+  case=> p1 => [a1 b1|a1 b1|q1 a1 b1|q1 a1 b1|q1 b1|q1 a1].
+  all: case=> p2 => [a2 b2|a2 b2|q2 a2 b2|q2 a2 b2|q2 b2|q2 a2] /= [] ??? ???; subst.
+  - intuition congruence.
+  - intuition congruence.
+  - move=> /(_ 0 0 2 0) H''P. exfalso. apply: H''P; by [|constructor|case|lia].
+  - move=> /(_ 0 0 1 1) H''P. exfalso. apply: H''P; by [|constructor|case|lia].
+  - intuition congruence.
+  - intuition congruence.
+  - intuition congruence.
+  - intuition congruence.
+  - move=> /(_ 0 0 1 1) H''P. exfalso. apply: H''P; by [|constructor|case|lia].
+  - move=> /(_ 0 0 0 2) H''P. exfalso. apply: H''P; by [|constructor|case|lia].
+  - intuition congruence.
+  - intuition congruence.
+  - move=> /(_ 2 0 0 0) H''P. exfalso. apply: H''P; by [|constructor|case|lia].
+  - move=> /(_ 1 1 0 0) H''P. exfalso. apply: H''P; by [|constructor|case|lia].
+  - have [|?] : p1 = p2 \/ p1 <> p2 by lia.
+    + intuition congruence.
+    + move=> /(_ 1 0 1 0) H''P. exfalso. apply: H''P; by [|constructor|case|lia].
+  - move=> /(_ 1 0 0 1) H''P. exfalso. apply: H''P; by [|constructor|case|lia].
+  - move=> /(_ 1 0 0 0) H''P. exfalso. apply: H''P; by [|constructor|case|lia].
+  - move=> /(_ 1 0 0 0) H''P. exfalso. apply: H''P; by [|constructor|case|lia].
+  - move=> /(_ 1 1 0 0) H''P. exfalso. apply: H''P; by [|constructor|case|lia].
+  - move=> /(_ 0 2 0 0) H''P. exfalso. apply: H''P; by [|constructor|case|lia].
+  - move=> /(_ 0 1 1 0) H''P. exfalso. apply: H''P; by [|constructor|case|lia].
+  - have [|?] : p1 = p2 \/ p1 <> p2 by lia.
+    + intuition congruence.
+    + move=> /(_ 0 1 0 1) H''P. exfalso. apply: H''P; by [|constructor|case|lia].
+  - move=> /(_ 0 1 0 0) H''P. exfalso. apply: H''P; by [|constructor|case|lia].
+  - move=> /(_ 0 1 0 0) H''P. exfalso. apply: H''P; by [|constructor|case|lia].
+  - intuition congruence.
+  - intuition congruence.
+  - move=> /(_ 0 0 1 0) H''P. exfalso. apply: H''P; by [|constructor|case|lia].
+  - move=> /(_ 0 0 0 1) H''P. exfalso. apply: H''P; by [|constructor|case|lia].
+  - intuition congruence.
+  - intuition congruence.
+  - intuition congruence.
+  - intuition congruence.
+  - move=> /(_ 0 0 1 0) H''P. exfalso. apply: H''P; by [|constructor|case|lia].
+  - move=> /(_ 0 0 0 1) H''P. exfalso. apply: H''P; by [|constructor|case|lia].
+  - intuition congruence.
+  - intuition congruence.
+Qed.
+
+(* informative decision statement for reversibility for mm2 *)
+Theorem decision : (mm2_reversible M) + (not (mm2_reversible M)).
+Proof.
+  pose t := list_prod (seq 1 l) (list_prod [0;1;2] [0;1;2]).
+  have := Forall_Exists_dec (fun '(x, y) => forall z, step x z -> step y z -> x = y) _ (list_prod t t).
+  apply: unnest.
+  { move=> [x y].
+    have [<-|?] := mm2_state_eq_dec x y.
+    { left. tauto. }
+    have [[z1 Hxz1]|Hx] := mm2_sig_step_dec M x.
+    - have [[z2 Hyz2]|Hy] := mm2_sig_step_dec M y.
+      + have [?|?] := mm2_state_eq_dec z2 z1.
+        * right. subst z2. by move=> /(_ z1 Hxz1 Hyz2).
+        * left => ?.
+          move: Hxz1 => /mm2_step_det /[apply] <-.
+          by move: Hyz2 => /mm2_step_det /[apply].
+      + by left => ?? /Hy.
+    - by left => ? /Hx. }
+  case.
+  { move=> /finite_characterization ?. by left. }
+  move=> H. right.
+  move: H => /Exists_exists [[x y]] [H'xy] Hxy HM. apply: Hxy.
+  by apply: HM.
+Qed.
+
+End Construction.
+
+Require Import Undecidability.Synthetic.Definitions.
+
+(* decision procedure for the reversibility of mm2 *)
+Definition decide : list mm2_instr -> bool :=
+  fun M =>
+    match decision M with
+    | inl _ => true
+    | inr _ => false
+    end.
+
+(* decision procedure correctness *)
+Lemma decide_spec : decider decide MM2_REV.
+Proof.
+  rewrite /decider /reflects /decide => M.
+  case: (decision M); [tauto | done].
+Qed.
